Risc0/Gadgets/IsZero/Constraints/CodeReordered.lean
@@ -10,8 +10,8 @@ open MLIRNotation
 def opt1 : MLIRProgram :=
   "%1" ←ₐ ⊤; "%2" ←ₐ .Get ⟨"in"⟩ 0 0; "%3" ←ₐ .Get ⟨"data"⟩ 0 0; "%4" ←ₐ ⟨"%1"⟩ &₀ ⟨"%2"⟩; "%5" ←ₐ guard ⟨"%3"⟩ & ⟨"%1"⟩ with ⟨"%4"⟩; "%0" ←ₐ .Const 1; "%6" ←ₐ .Sub ⟨"%0"⟩ ⟨"%3"⟩; "%7" ←ₐ .Get ⟨"data"⟩ 0 1; "%8" ←ₐ .Mul ⟨"%2"⟩ ⟨"%7"⟩; "%9" ←ₐ .Sub ⟨"%8"⟩ ⟨"%0"⟩; "%10" ←ₐ ⟨"%1"⟩ &₀ ⟨"%9"⟩; "%11" ←ₐ guard ⟨"%6"⟩ & ⟨"%5"⟩ with ⟨"%10"⟩
 lemma optimised_behaviour1 :
-  getReturn (full.runProgram st) =
-  getReturn (opt1.runProgram st) := by
+  getReturn (full.runProgram st)  =
+  getReturn (opt1.runProgram st)  := by
     unfold getReturn MLIR.runProgram full
     rewrite[opt_swap (const_past_true (by trivial)),opt_swap (const_past_get (by trivial)),opt_swap (const_past_get (by trivial)),opt_swap (const_past_andEqz (by trivial)),opt_swap (const_past_andCond (by trivial))]
     simp only [←MLIR.run_nondet]
@@ -23,8 +23,8 @@ lemma optimised_behaviour1 :
 def opt2 : MLIRProgram :=
   "%1" ←ₐ ⊤; "%3" ←ₐ .Get ⟨"data"⟩ 0 0; "%2" ←ₐ .Get ⟨"in"⟩ 0 0; "%4" ←ₐ ⟨"%1"⟩ &₀ ⟨"%2"⟩; "%5" ←ₐ guard ⟨"%3"⟩ & ⟨"%1"⟩ with ⟨"%4"⟩; "%0" ←ₐ .Const 1; "%6" ←ₐ .Sub ⟨"%0"⟩ ⟨"%3"⟩; "%7" ←ₐ .Get ⟨"data"⟩ 0 1; "%8" ←ₐ .Mul ⟨"%2"⟩ ⟨"%7"⟩; "%9" ←ₐ .Sub ⟨"%8"⟩ ⟨"%0"⟩; "%10" ←ₐ ⟨"%1"⟩ &₀ ⟨"%9"⟩; "%11" ←ₐ guard ⟨"%6"⟩ & ⟨"%5"⟩ with ⟨"%10"⟩
 lemma optimised_behaviour2 :
-  getReturn (full.runProgram st) =
-  getReturn (opt2.runProgram st) := by
+  getReturn (full.runProgram st)  =
+  getReturn (opt2.runProgram st)  := by
     rewrite [optimised_behaviour1]
     unfold getReturn MLIR.runProgram opt1
     rewrite[MLIR.run_seq_def]
@@ -38,8 +38,8 @@ lemma optimised_behaviour2 :
 def opt3 : MLIRProgram :=
   "%1" ←ₐ ⊤; "%2" ←ₐ .Get ⟨"in"⟩ 0 0; "%4" ←ₐ ⟨"%1"⟩ &₀ ⟨"%2"⟩; "%3" ←ₐ .Get ⟨"data"⟩ 0 0; "%5" ←ₐ guard ⟨"%3"⟩ & ⟨"%1"⟩ with ⟨"%4"⟩; "%0" ←ₐ .Const 1; "%6" ←ₐ .Sub ⟨"%0"⟩ ⟨"%3"⟩; "%7" ←ₐ .Get ⟨"data"⟩ 0 1; "%8" ←ₐ .Mul ⟨"%2"⟩ ⟨"%7"⟩; "%9" ←ₐ .Sub ⟨"%8"⟩ ⟨"%0"⟩; "%10" ←ₐ ⟨"%1"⟩ &₀ ⟨"%9"⟩; "%11" ←ₐ guard ⟨"%6"⟩ & ⟨"%5"⟩ with ⟨"%10"⟩
 lemma optimised_behaviour3 :
-  getReturn (full.runProgram st) =
-  getReturn (opt3.runProgram st) := by
+  getReturn (full.runProgram st)  =
+  getReturn (opt3.runProgram st)  := by
     rewrite [optimised_behaviour2]
     unfold getReturn MLIR.runProgram opt2
     rewrite[MLIR.run_seq_def]
@@ -53,8 +53,8 @@ lemma optimised_behaviour3 :
 def opt_full : MLIRProgram := opt3
 lemma opt_full_def : opt_full = opt3 := rfl
 lemma optimised_behaviour_full :
-  getReturn (full.runProgram st) =
-  getReturn (opt_full.runProgram st) := by
+  getReturn (full.runProgram st)  =
+  getReturn (opt_full.runProgram st)  := by
   rewrite [optimised_behaviour3]
   rw [opt_full]
 end Risc0.IsZero.Constraints.Code
